Primitive_Matchers/Iface.thy
@@ -58,4 +58,5 @@ fun match_iface :: "iface \<Rightarrow> string \<Rightarrow> bool" where
   "match_iface (Iface (Pos i)) p_iface \<longleftrightarrow> cmp_iface_name p_iface i" |
   "match_iface (Iface (Neg i)) p_iface \<longleftrightarrow> \<not> cmp_iface_name p_iface i"
 
+
 end
